skip_list/arrays/inv/lazy_inv.v
@@ -30,7 +30,7 @@ Module LazyListInv (Params: SKIP_LIST_PARAMS).
   Export ListEquiv.
 
   Section Proofs.
-    Context `{!heapGS Σ, !gset_list_unionGS Σ, !lockG Σ} (lvl: nat).
+    Context `{!heapGS Σ, !gset_list_unionGS Σ, !lockG Σ} (lvl: Z).
 
     Definition from_sub_list (obot: option sub_gname) (rep: node_rep) : iProp Σ := 
       match obot with
@@ -75,7 +75,7 @@ Module LazyListInv (Params: SKIP_LIST_PARAMS).
       | Some bot => bot_list_inv bot Skeys
       end.
 
-    Definition levelN (lvl: nat) := nroot .@ "level" .@ lvl.
+    Definition levelN (lvl: Z) := nroot .@ "level" .@ lvl.
 
     Definition is_top_list (head: node_rep) (top bot: sub_gname) : iProp Σ := 
       inv (levelN lvl) (lazy_list_inv head top None (from_top_list bot)).
