skip_list/arrays/spec/add.v
@@ -19,25 +19,25 @@ Module AddSpec (Params: SKIP_LIST_PARAMS).
   Section Proofs.
     Context `{!heapGS Σ, !gset_list_unionGS Σ, !lockG Σ}.
 
-    Theorem topLevel_spec (lvl h: nat) (key: Z) (top_head curr: node_rep) (S: gset Z) (q: frac)
+    Theorem topLevel_spec (key h lvl: Z) (top_head curr: node_rep) (Skeys: gset Z) (q: frac)
       (bot: bot_gname) (top_sub: sub_gname) (bot_subs: list sub_gname) :
       {{{
-        skip_list_equiv lvl top_head S q bot (top_sub :: bot_subs)
+        skip_list_equiv lvl top_head Skeys q bot (top_sub :: bot_subs)
         ∗
         (⌜ curr = top_head ⌝ ∨ own (s_auth top_sub) (◯ {[ curr ]}))
         ∗
         ⌜ node_key curr < key < INT_MAX ⌝
         ∗
-        ⌜ h ≤ lvl ⌝
+        ⌜ 0 ≤ h ≤ lvl ⌝
       }}}
         topLevel (rep_to_node curr) #key #h #lvl
       {{{ curr' top_head' top_sub' bot_subs', RET rep_to_node curr';
-        skip_list_equiv h top_head' S q bot (top_sub' :: bot_subs')
+        skip_list_equiv h top_head' Skeys q bot (top_sub' :: bot_subs')
         ∗
         ( 
-          skip_list_equiv h top_head' (S ∪ {[ key ]}) q bot (top_sub' :: bot_subs')
+          skip_list_equiv h top_head' (Skeys ∪ {[ key ]}) q bot (top_sub' :: bot_subs')
           -∗
-          skip_list_equiv lvl top_head (S ∪ {[ key ]}) q bot (top_sub :: bot_subs)
+          skip_list_equiv lvl top_head (Skeys ∪ {[ key ]}) q bot (top_sub :: bot_subs)
         )
         ∗
         (⌜ curr' = top_head' ⌝ ∨ own (s_auth top_sub') (◯ {[ curr' ]}))
@@ -60,8 +60,7 @@ Module AddSpec (Params: SKIP_LIST_PARAMS).
       iIntros (pred succ) "(%Hrange' & #Hown_pred & #Hown_succ & _)".
       wp_pures.
       case_bool_decide as Hcase; wp_if.
-      + inversion Hcase as [Heq]. 
-        assert (h = lvl)%nat as <- by lia.
+      + assert (h = lvl) as <- by congruence.
         iModIntro; iApply "HΦ". 
         iFrame "# ∗". 
         iSplit; last (iPureIntro; lia).
@@ -72,16 +71,15 @@ Module AddSpec (Params: SKIP_LIST_PARAMS).
         iDestruct "Hlist" as "(#Hlvl & #Hinv & Hmatch)"; unfold is_top_list.
 
         wp_bind (BinOp _ _ _).
-        iInv (levelN lvl) as (S' Skeys L) "(Hinv_sub & _)" "Hclose".
+        iInv (levelN lvl) as (S' Skeys' L) "(Hinv_sub & _)" "Hclose".
         iDestruct "Hinv_sub" as "(>%Hperm & >%Hsort & >%Hequiv & >Hown_auth & >Hown_toks & Hlist)".
 
         iDestruct "Hown_pred" as "[%Heq | #Hown_pred]".
         - wp_op.
           iMod ("Hclose" with "[Hlist Hown_auth Hown_toks]") as "_".
-          { iNext; iExists S', Skeys, L; by iFrame. }
+          { iNext; iExists S', Skeys', L; by iFrame. }
           iModIntro.
 
-          assert (lvl - 1 = (lvl - 1)%nat) as -> by lia.
           iApply ("IH" with "[$] [] [%] [%]").
           { by iLeft. }
           { lia. }
@@ -105,10 +103,9 @@ Module AddSpec (Params: SKIP_LIST_PARAMS).
           wp_op.
           iPoseProof ("Himp" with "[$]") as "Hlist".
           iMod ("Hclose" with "[Hlist Hown_auth Hown_toks]") as "_".
-          { iNext; iExists S', Skeys, L; by iFrame. }
+          { iNext; iExists S', Skeys', L; by iFrame. }
           iModIntro.
         
-          assert (lvl - 1 = (lvl - 1)%nat) as -> by lia.
           iApply ("IH" with "[$] [$] [%] [%]").
           { lia. }
           { lia. }
@@ -119,7 +116,7 @@ Module AddSpec (Params: SKIP_LIST_PARAMS).
           iApply "HΦ". iFrame "# ∗".
     Qed.
 
-    Theorem addAll_spec (lvl h: nat) (key: Z) (top_head curr: node_rep) (Skeys: gset Z) (q: frac)
+    Theorem addAll_spec (key h lvl: Z) (top_head curr: node_rep) (Skeys: gset Z) (q: frac)
       (bot: bot_gname) (top_sub: sub_gname) (bot_subs: list sub_gname) :
       INT_MIN < key < INT_MAX →
       {{{
@@ -129,7 +126,7 @@ Module AddSpec (Params: SKIP_LIST_PARAMS).
         ∗
         ⌜ node_key curr < key ⌝
         ∗
-        ⌜ lvl ≤ h ⌝
+        ⌜ 0 ≤ lvl ≤ h ⌝
       }}}
         addAll (rep_to_node curr) #key #h #lvl
       {{{ (v: val) (n: loc) (new: node_rep), RET v;
@@ -150,12 +147,12 @@ Module AddSpec (Params: SKIP_LIST_PARAMS).
             ∗ 
             n ↦{#lfrac lvl} rep_to_node new
             ∗
-            (node_next new +ₗ lvl +ₗ 1) ↦∗{#1 / 2} replicate (h - lvl) #()
+            (node_next new +ₗ lvl +ₗ 1) ↦∗{#1 / 2} replicate (Z.to_nat (h - lvl)) #()
             ∗
             ∃ (γ: gname), 
-              is_lock γ (node_lock new) (in_lock (node_next new) (S h))
+              is_lock γ (node_lock new) (in_lock (node_next new) (h + 1))
               ∗
-              in_lock (node_next new) (S h)
+              in_lock (node_next new) (h + 1)
               ∗
               locked γ
           )
@@ -182,19 +179,13 @@ Module AddSpec (Params: SKIP_LIST_PARAMS).
         wp_apply (tryInsert_spec with "[Hown_frag]").
         { done. }
         { iFrame "# ∗". iPureIntro; lia. }
-
         iIntros (v n new) "((Hown_frac & _) & Hopt)".
+
         iApply "HΦ". 
         rewrite loc_add_0.
-        assert (h - 0 = h)%nat as -> by lia.
-
-        assert (1 / 2 / 2 = lfrac 0%nat)%Qp as ->.
-        {
-          rewrite /lfrac.
-          assert (0 + 2 = 2)%nat as -> by lia.
-          rewrite /= Qp_mul_1_r -Qp_div_div //.
-        }
-
+        assert (h - 0 = h) as -> by lia.
+        assert (1 / 2 / 2 = lfrac 0)%Qp as ->.
+        { rewrite /lfrac /= Qp_mul_1_r -Qp_div_div //. }
         by iFrame "# ∗".
       + iDestruct "Hlist" as "(%Hlvl & #Hinv & Hmatch)"; unfold is_top_list.
         case_bool_decide as Hcase; wp_if.
@@ -210,7 +201,6 @@ Module AddSpec (Params: SKIP_LIST_PARAMS).
             iModIntro. 
 
             wp_bind (addAll _ _ _ _).
-            assert (lvl - 1 = (lvl - 1)%nat) as -> by lia.
             iApply ("IH" with "[$] [] [%] [%]").
             { by iLeft. }
             { lia. }
@@ -224,30 +214,30 @@ Module AddSpec (Params: SKIP_LIST_PARAMS).
                iSplitR ""; last by iLeft.
                by iFrame "# ∗".
             ++ rewrite Hopt. wp_pures.
-
                iDestruct "Hn" as "(Hn & Hn')".
                assert (lfrac (lvl - 1) / 2 = lfrac lvl)%Qp as ->.
                {
                  rewrite /lfrac.
-                 assert (lvl - 1 + 2 = S lvl)%nat as -> by lia.
-                 assert (lvl + 2 = S (S lvl))%nat as -> by lia.
+                 assert (Z.to_nat (lvl - 1) + 2 = S (Z.to_nat lvl))%nat as -> by lia.
+                 assert (Z.to_nat lvl + 2 = S (S (Z.to_nat lvl)))%nat as -> by lia.
                  rewrite /= Qp_div_div Qp_mul_comm //.
                }
 
                rewrite loc_add_assoc.
-               assert ((lvl - 1)%nat + 1 = lvl) as -> by lia.
-               assert (h - (lvl - 1) = S (h - lvl))%nat as -> by lia.
+               assert (Z.to_nat (h - (lvl - 1)) = S (Z.to_nat (h - lvl)))%nat as -> by lia.
                rewrite replicate_S array_cons.
                iDestruct "Hnext" as "(Hnext & Hreplicate)".
 
                iDestruct "Hlock" as (γ) "(#Hlock & Hin_lock & Hlocked)".
                iDestruct "Hin_lock" as (vs) "(Hnext' & %Hlength)".
-               pose proof (list_split vs h lvl) as Hsplit.
+               pose proof (list_split vs (Z.to_nat h) (Z.to_nat lvl)) as Hsplit.
                destruct Hsplit as [next Hsplit]; try lia.
                destruct Hsplit as [vs1 Hsplit]; destruct Hsplit as [vs2 Hsplit].
                destruct Hsplit as [Hvs Hsplit]; destruct Hsplit as [Hlength1 Hlength2].
                rewrite Hvs array_app array_cons Hlength1.
                iDestruct "Hnext'" as "(Hnext'1 & Hnext' & Hnext'2)".
+               assert (lvl = Z.to_nat lvl) as <- by lia.
+               assert (lvl - 1 + 1 = lvl) as -> by lia.
                iDestruct (mapsto_agree with "Hnext Hnext'") as %<-.
                iCombine "Hnext Hnext'" as "Hnext".
 
@@ -268,6 +258,7 @@ Module AddSpec (Params: SKIP_LIST_PARAMS).
                iExists γ. iFrame "# ∗".
 
                iCombine "Hnext'1 Hnext Hnext'2" as "Hnext".
+               assert (lvl = Z.to_nat lvl) as -> by lia.
                rewrite -array_cons -Hlength1 -array_app.
                iExists (vs1 ++ #n' :: vs2); iFrame.
                iPureIntro; rewrite app_length cons_length; lia.
@@ -290,7 +281,6 @@ Module AddSpec (Params: SKIP_LIST_PARAMS).
             iModIntro.
           
             wp_bind (addAll _ _ _ _).
-            assert (lvl - 1 = (lvl - 1)%nat) as -> by lia.
             iApply ("IH" with "[$] [$] [%] [%]").
             { lia. }
             { lia. }
@@ -308,25 +298,26 @@ Module AddSpec (Params: SKIP_LIST_PARAMS).
                assert (lfrac (lvl - 1) / 2 = lfrac lvl)%Qp as ->.
                {
                  rewrite /lfrac.
-                 assert (lvl - 1 + 2 = S lvl)%nat as -> by lia.
-                 assert (lvl + 2 = S (S lvl))%nat as -> by lia.
+                 assert (Z.to_nat (lvl - 1) + 2 = S (Z.to_nat lvl))%nat as -> by lia.
+                 assert (Z.to_nat lvl + 2 = S (S (Z.to_nat lvl)))%nat as -> by lia.
                  rewrite /= Qp_div_div Qp_mul_comm //.
                }
 
                rewrite loc_add_assoc.
-               assert ((lvl - 1)%nat + 1 = lvl) as -> by lia.
-               assert (h - (lvl - 1) = S (h - lvl))%nat as -> by lia.
+               assert (Z.to_nat (h - (lvl - 1)) = S (Z.to_nat (h - lvl)))%nat as -> by lia.
                rewrite replicate_S array_cons.
                iDestruct "Hnext" as "(Hnext & Hreplicate)".
 
                iDestruct "Hlock" as (γ) "(#Hlock & Hin_lock & Hlocked)".
                iDestruct "Hin_lock" as (vs) "(Hnext' & %Hlength)".
-               pose proof (list_split vs h lvl) as Hsplit.
+               pose proof (list_split vs (Z.to_nat h) (Z.to_nat lvl)) as Hsplit.
                destruct Hsplit as [next Hsplit]; try lia.
                destruct Hsplit as [vs1 Hsplit]; destruct Hsplit as [vs2 Hsplit].
                destruct Hsplit as [Hvs Hsplit]; destruct Hsplit as [Hlength1 Hlength2].
                rewrite Hvs array_app array_cons Hlength1.
                iDestruct "Hnext'" as "(Hnext'1 & Hnext' & Hnext'2)".
+               assert (lvl = Z.to_nat lvl) as <- by lia.
+               assert (lvl - 1 + 1 = lvl) as -> by lia.
                iDestruct (mapsto_agree with "Hnext Hnext'") as %<-.
                iCombine "Hnext Hnext'" as "Hnext".
 
@@ -343,15 +334,16 @@ Module AddSpec (Params: SKIP_LIST_PARAMS).
                iExists γ. iFrame "# ∗".
                
                iCombine "Hnext'1 Hnext Hnext'2" as "Hnext".
+               assert (lvl = Z.to_nat lvl) as -> by lia.
                rewrite -array_cons -Hlength1 -array_app.
                iExists (vs1 ++ #n' :: vs2); iFrame.
                iPureIntro; rewrite app_length cons_length; lia.
     Qed.
 
-    Theorem add_spec (key: Z) (height: nat) (v: val) (S: gset Z) (q: frac)
+    Theorem add_spec (key height: Z) (v: val) (S: gset Z) (q: frac)
       (bot: bot_gname) (subs: list sub_gname)
       (Hrange: INT_MIN < key < INT_MAX) 
-      (Hheight: height ≤ MAX_HEIGHT) :
+      (Hheight: 0 ≤ height ≤ MAX_HEIGHT) :
       {{{ is_skip_list v S q bot subs }}}
         add v #key #height
       {{{ (b: bool), RET #b; is_skip_list v (S ∪ {[ key ]}) q bot subs }}}.
